src/Std/Data/DHashMap/RawLemmas.lean
@@ -39,7 +39,7 @@ private def baseNames : Array Name :=
     ``getThenInsertIfNew?_snd_eq, ``getThenInsertIfNew?_snd_val,
     ``map_eq, ``map_val,
     ``filter_eq, ``filter_val,
-    ``remove_eq, ``remove_val,
+    ``erase_eq, ``erase_val,
     ``filterMap_eq, ``filterMap_val,
     ``Const.getThenInsertIfNew?_snd_eq, ``Const.getThenInsertIfNew?_snd_val,
     ``containsThenInsert_fst_eq, ``containsThenInsert_fst_val,
@@ -158,42 +158,42 @@ theorem size_le_size_insert [EquivBEq α] [LawfulHashable α] {k : α} {v : β k
   simp_to_raw using Raw₀.size_le_size_insert ⟨m, _⟩ h
 
 @[simp]
-theorem remove_empty {k : α} {c : Nat} : (empty c : Raw α β).remove k = empty c := by
-  rw [remove_eq (by wf_trivial)]
-  exact congrArg Subtype.val Raw₀.remove_empty
+theorem erase_empty {k : α} {c : Nat} : (empty c : Raw α β).erase k = empty c := by
+  rw [erase_eq (by wf_trivial)]
+  exact congrArg Subtype.val Raw₀.erase_empty
 
 @[simp]
-theorem remove_emptyc {k : α} : (∅ : Raw α β).remove k = ∅ :=
-  remove_empty
+theorem erase_emptyc {k : α} : (∅ : Raw α β).erase k = ∅ :=
+  erase_empty
 
 @[simp]
-theorem isEmpty_remove [EquivBEq α] [LawfulHashable α] {k : α} :
-    (m.remove k).isEmpty = (m.isEmpty || (m.size == 1 && m.contains k)) := by
-  simp_to_raw using Raw₀.isEmpty_remove
+theorem isEmpty_erase [EquivBEq α] [LawfulHashable α] {k : α} :
+    (m.erase k).isEmpty = (m.isEmpty || (m.size == 1 && m.contains k)) := by
+  simp_to_raw using Raw₀.isEmpty_erase
 
 @[simp]
-theorem contains_remove [EquivBEq α] [LawfulHashable α] {k a : α} :
-    (m.remove k).contains a = (!(k == a) && m.contains a) := by
-  simp_to_raw using Raw₀.contains_remove
+theorem contains_erase [EquivBEq α] [LawfulHashable α] {k a : α} :
+    (m.erase k).contains a = (!(k == a) && m.contains a) := by
+  simp_to_raw using Raw₀.contains_erase
 
 @[simp]
-theorem mem_remove [EquivBEq α] [LawfulHashable α] {k a : α} :
-    a ∈ m.remove k ↔ (k == a) = false ∧ a ∈ m := by
-  simp [mem_iff_contains, contains_remove h]
+theorem mem_erase [EquivBEq α] [LawfulHashable α] {k a : α} :
+    a ∈ m.erase k ↔ (k == a) = false ∧ a ∈ m := by
+  simp [mem_iff_contains, contains_erase h]
 
-theorem contains_of_contains_remove [EquivBEq α] [LawfulHashable α] {k a : α} :
-    (m.remove k).contains a → m.contains a := by
-  simp_to_raw using Raw₀.contains_of_contains_remove
+theorem contains_of_contains_erase [EquivBEq α] [LawfulHashable α] {k a : α} :
+    (m.erase k).contains a → m.contains a := by
+  simp_to_raw using Raw₀.contains_of_contains_erase
 
-theorem mem_of_mem_remove [EquivBEq α] [LawfulHashable α] {k a : α} : a ∈ m.remove k → a ∈ m := by
-  simpa [mem_iff_contains] using contains_of_contains_remove h
+theorem mem_of_mem_erase [EquivBEq α] [LawfulHashable α] {k a : α} : a ∈ m.erase k → a ∈ m := by
+  simpa [mem_iff_contains] using contains_of_contains_erase h
 
-theorem size_remove [EquivBEq α] [LawfulHashable α] {k : α} :
-    (m.remove k).size = bif m.contains k then m.size - 1 else m.size := by
-  simp_to_raw using Raw₀.size_remove
+theorem size_erase [EquivBEq α] [LawfulHashable α] {k : α} :
+    (m.erase k).size = bif m.contains k then m.size - 1 else m.size := by
+  simp_to_raw using Raw₀.size_erase
 
-theorem size_remove_le [EquivBEq α] [LawfulHashable α] {k : α} : (m.remove k).size ≤ m.size := by
-  simp_to_raw using Raw₀.size_remove_le
+theorem size_erase_le [EquivBEq α] [LawfulHashable α] {k : α} : (m.erase k).size ≤ m.size := by
+  simp_to_raw using Raw₀.size_erase_le
 
 @[simp]
 theorem containsThenInsert_fst {k : α} {v : β k} : (m.containsThenInsert k v).1 = m.contains k := by
@@ -242,13 +242,13 @@ theorem get?_eq_none_of_contains_eq_false [LawfulBEq α] {a : α} :
 theorem get?_eq_none [LawfulBEq α] {a : α} : ¬a ∈ m → m.get? a = none := by
   simpa [mem_iff_contains] using get?_eq_none_of_contains_eq_false h
 
-theorem get?_remove [LawfulBEq α] {k a : α} :
-    (m.remove k).get? a = bif k == a then none else m.get? a := by
-  simp_to_raw using Raw₀.get?_remove
+theorem get?_erase [LawfulBEq α] {k a : α} :
+    (m.erase k).get? a = bif k == a then none else m.get? a := by
+  simp_to_raw using Raw₀.get?_erase
 
 @[simp]
-theorem get?_remove_self [LawfulBEq α] {k : α} : (m.remove k).get? k = none := by
-  simp_to_raw using Raw₀.get?_remove_self
+theorem get?_erase_self [LawfulBEq α] {k : α} : (m.erase k).get? k = none := by
+  simp_to_raw using Raw₀.get?_erase_self
 
 namespace Const
 
@@ -286,13 +286,13 @@ theorem get?_eq_none_of_contains_eq_false [EquivBEq α] [LawfulHashable α] {a :
 theorem get?_eq_none [EquivBEq α] [LawfulHashable α] {a : α} : ¬a ∈ m → get? m a = none := by
     simpa [mem_iff_contains] using get?_eq_none_of_contains_eq_false h
 
-theorem get?_remove [EquivBEq α] [LawfulHashable α] {k a : α} :
-    Const.get? (m.remove k) a = bif k == a then none else get? m a := by
-  simp_to_raw using Raw₀.Const.get?_remove
+theorem get?_erase [EquivBEq α] [LawfulHashable α] {k a : α} :
+    Const.get? (m.erase k) a = bif k == a then none else get? m a := by
+  simp_to_raw using Raw₀.Const.get?_erase
 
 @[simp]
-theorem get?_remove_self [EquivBEq α] [LawfulHashable α] {k : α} : get? (m.remove k) k = none := by
-  simp_to_raw using Raw₀.Const.get?_remove_self
+theorem get?_erase_self [EquivBEq α] [LawfulHashable α] {k : α} : get? (m.erase k) k = none := by
+  simp_to_raw using Raw₀.Const.get?_erase_self
 
 theorem get?_eq_get? [LawfulBEq α] {a : α} : get? m a = m.get? a := by
   simp_to_raw using Raw₀.Const.get?_eq_get?
@@ -317,9 +317,9 @@ theorem get_insert_self [LawfulBEq α] {k : α} {v : β k} :
   simp_to_raw using Raw₀.get_insert_self ⟨m, _⟩
 
 @[simp]
-theorem get_remove [LawfulBEq α] {k a : α} {h'} :
-    (m.remove a).get k h' = m.get k (mem_of_mem_remove h h') := by
-  simp_to_raw using Raw₀.get_remove ⟨m, _⟩
+theorem get_erase [LawfulBEq α] {k a : α} {h'} :
+    (m.erase a).get k h' = m.get k (mem_of_mem_erase h h') := by
+  simp_to_raw using Raw₀.get_erase ⟨m, _⟩
 
 theorem get?_eq_some_get [LawfulBEq α] {a : α} {h} : m.get? a = some (m.get a h) := by
   simp_to_raw using Raw₀.get?_eq_some_get
@@ -339,9 +339,9 @@ theorem get_insert_self [EquivBEq α] [LawfulHashable α] {k : α} {v : β} :
   simp_to_raw using Raw₀.Const.get_insert_self ⟨m, _⟩
 
 @[simp]
-theorem get_remove [EquivBEq α] [LawfulHashable α] {k a : α} {h'} :
-    get (m.remove k) a h' = get m a (mem_of_mem_remove h h') := by
-  simp_to_raw using Raw₀.Const.get_remove ⟨m, _⟩
+theorem get_erase [EquivBEq α] [LawfulHashable α] {k a : α} {h'} :
+    get (m.erase k) a h' = get m a (mem_of_mem_erase h h') := by
+  simp_to_raw using Raw₀.Const.get_erase ⟨m, _⟩
 
 theorem get?_eq_some_get [EquivBEq α] [LawfulHashable α] {a : α} {h : a ∈ m} :
     get? m a = some (get m a h) := by
@@ -387,14 +387,14 @@ theorem get!_eq_default [LawfulBEq α] {a : α} [Inhabited (β a)] :
     ¬a ∈ m → m.get! a = default := by
   simpa [mem_iff_contains] using get!_eq_default_of_contains_eq_false h
 
-theorem get!_remove [LawfulBEq α] {k a : α} [Inhabited (β a)] :
-    (m.remove k).get! a = bif k == a then default else m.get! a := by
-  simp_to_raw using Raw₀.get!_remove
+theorem get!_erase [LawfulBEq α] {k a : α} [Inhabited (β a)] :
+    (m.erase k).get! a = bif k == a then default else m.get! a := by
+  simp_to_raw using Raw₀.get!_erase
 
 @[simp]
-theorem get!_remove_self [LawfulBEq α] {k : α} [Inhabited (β k)] :
-    (m.remove k).get! k = default := by
-  simp_to_raw using Raw₀.get!_remove_self
+theorem get!_erase_self [LawfulBEq α] {k : α} [Inhabited (β k)] :
+    (m.erase k).get! k = default := by
+  simp_to_raw using Raw₀.get!_erase_self
 
 theorem get?_eq_some_get!_of_contains [LawfulBEq α] {a : α} [Inhabited (β a)] :
     m.contains a = true → m.get? a = some (m.get! a) := by
@@ -445,14 +445,14 @@ theorem get!_eq_default [EquivBEq α] [LawfulHashable α] [Inhabited β] {a : α
     ¬a ∈ m → get! m a = default := by
   simpa [mem_iff_contains] using get!_eq_default_of_contains_eq_false h
 
-theorem get!_remove [EquivBEq α] [LawfulHashable α] [Inhabited β] {k a : α} :
-    get! (m.remove k) a = bif k == a then default else get! m a := by
-  simp_to_raw using Raw₀.Const.get!_remove
+theorem get!_erase [EquivBEq α] [LawfulHashable α] [Inhabited β] {k a : α} :
+    get! (m.erase k) a = bif k == a then default else get! m a := by
+  simp_to_raw using Raw₀.Const.get!_erase
 
 @[simp]
-theorem get!_remove_self [EquivBEq α] [LawfulHashable α] [Inhabited β] {k : α} :
-    get! (m.remove k) k = default := by
-  simp_to_raw using Raw₀.Const.get!_remove_self
+theorem get!_erase_self [EquivBEq α] [LawfulHashable α] [Inhabited β] {k : α} :
+    get! (m.erase k) k = default := by
+  simp_to_raw using Raw₀.Const.get!_erase_self
 
 theorem get?_eq_some_get!_of_contains [EquivBEq α] [LawfulHashable α] [Inhabited β] {a : α} :
     m.contains a = true → get? m a = some (get! m a) := by
@@ -512,14 +512,14 @@ theorem getD_eq_fallback [LawfulBEq α] {a : α} {fallback : β a} :
     ¬a ∈ m → m.getD a fallback = fallback := by
   simpa [mem_iff_contains] using getD_eq_fallback_of_contains_eq_false h
 
-theorem getD_remove [LawfulBEq α] {k a : α} {fallback : β a} :
-    (m.remove k).getD a fallback = bif k == a then fallback else m.getD a fallback := by
-  simp_to_raw using Raw₀.getD_remove
+theorem getD_erase [LawfulBEq α] {k a : α} {fallback : β a} :
+    (m.erase k).getD a fallback = bif k == a then fallback else m.getD a fallback := by
+  simp_to_raw using Raw₀.getD_erase
 
 @[simp]
-theorem getD_remove_self [LawfulBEq α] {k : α} {fallback : β k} :
-    (m.remove k).getD k fallback = fallback := by
-  simp_to_raw using Raw₀.getD_remove_self
+theorem getD_erase_self [LawfulBEq α] {k : α} {fallback : β k} :
+    (m.erase k).getD k fallback = fallback := by
+  simp_to_raw using Raw₀.getD_erase_self
 
 theorem get?_eq_some_getD_of_contains [LawfulBEq α] {a : α} {fallback : β a} :
     m.contains a = true → m.get? a = some (m.getD a fallback) := by
@@ -575,14 +575,14 @@ theorem getD_eq_fallback [EquivBEq α] [LawfulHashable α] {a : α} {fallback : 
     ¬a ∈ m → getD m a fallback = fallback := by
   simpa [mem_iff_contains] using getD_eq_fallback_of_contains_eq_false h
 
-theorem getD_remove [EquivBEq α] [LawfulHashable α] {k a : α} {fallback : β} :
-    getD (m.remove k) a fallback = bif k == a then fallback else getD m a fallback := by
-  simp_to_raw using Raw₀.Const.getD_remove
+theorem getD_erase [EquivBEq α] [LawfulHashable α] {k a : α} {fallback : β} :
+    getD (m.erase k) a fallback = bif k == a then fallback else getD m a fallback := by
+  simp_to_raw using Raw₀.Const.getD_erase
 
 @[simp]
-theorem getD_remove_self [EquivBEq α] [LawfulHashable α] {k : α} {fallback : β} :
-    getD (m.remove k) k fallback = fallback := by
-  simp_to_raw using Raw₀.Const.getD_remove_self
+theorem getD_erase_self [EquivBEq α] [LawfulHashable α] {k : α} {fallback : β} :
+    getD (m.erase k) k fallback = fallback := by
+  simp_to_raw using Raw₀.Const.getD_erase_self
 
 theorem get?_eq_some_getD_of_contains [EquivBEq α] [LawfulHashable α] {a : α} {fallback : β} :
     m.contains a = true → get? m a = some (getD m a fallback) := by
